\documentclass{beamer}
\setbeamertemplate{navigation symbols}{}

\usepackage{amsmath}
\usepackage{hyperref}
\usetheme{Montpellier}


\beamersetuncovermixins{\opaqueness<1>{25}}{\opaqueness<2->{15}}
\begin{document}
\title{LU Decomposition}  
\author{By\\ Dilip Puri\\Govind Meena\\Hemant Kumar}
\date{\today} 
\begin{frame}
\titlepage
\end{frame}

%\begin{frame}\frametitle{Table of contents}\tableofcontents
%\end{frame} 

\section{Problem} 
\begin{frame}\frametitle{Problem} 
We have a matrix A, now we want to decompose matrix A into two matrices L(Lower Triangular Matrix) and U(Upper Triangular Matrix) such that \\
\begin{center}
\begin{LARGE}
\textbf{A = L * U}\\
where
\begin{equation*}
L = \left[ \begin{aligned}
1 && 0 && 0 \\
a && 1 && 0 \\
b && c && 1
\end{aligned}
\right]\,,
U = \left[ \begin{aligned}
d && e && f \\
0 && g && h \\
0 && 0 && i
\end{aligned}
\right]\,.
\end{equation*}
\end{LARGE}
\end{center}
\end{frame}


\section{Motivation} 
\begin{frame}\frametitle{Motivation} 
\texttt{So the first question come to mind that why we are doing this?}\\
so straight forward answer would be that it will simplify things. How?\\
Most of the time in mathematics modeling we came up with system of linear equations in the form of\\
\begin{center}
\begin{LARGE}
\textbf{Ax = b}
\end{LARGE}
\end{center}
so finding $A^{-1}$ is quite difficult so we will use LU decomposition\\
\begin{center} \begin{huge}
How?
\end{huge} \end{center}
\end{frame}

\begin{frame}{Example}
Lets we have system of eqations
\begin{align*}
  [A]\{x\} = \{b\}\\
  	[L][U]\{x\} = \{b\}\\
  	(\therefore [A] = [L][U])\\
  \{y\} = [U]\{x\}\\
  [L]\{y\} = \{b\}\\
  \because []=matrix, \{\}=vector
\end{align*}
This will make our system so simple to solve...
\end{frame}

\begin{frame}{Example}
\begin{equation*}
A = \left[ \begin{aligned}
1 && 2 && 4 \\
3 && 8 && 14 \\
2 && 6 && 13
\end{aligned}
\right]\,,
x = \left[ \begin{aligned}
x_1\\
x_2\\
x_3
\end{aligned}
\right]\,,
b = \left[ \begin{aligned}
3\\
13\\
4
\end{aligned}
\right]\,.
\end{equation*}
\begin{equation*}
A= LU \Rightarrow \left[ \begin{aligned}
1 && 0 && 0 \\
a && 1 && 0 \\
b && c && 1
\end{aligned}
\right]\,*
\left[ \begin{aligned}
d && e && f \\
0 && g && h \\
0 && 0 && i
\end{aligned}
\right]\,=
\left[ \begin{aligned}
d && e && f \\
ad && ae+g && af+h \\
bd && be+cg && bf+ch+i
\end{aligned}
\right]\,.
\end{equation*}
\begin{equation*}
\Rightarrow
\left[ \begin{aligned}
d && e && f \\
ad && ae+g && af+h \\
bd && be+cg && bf+ch+i
\end{aligned}
\right]\,=
\left[ \begin{aligned}
1 && 2 && 4 \\
3 && 8 && 14 \\
2 && 6 && 13
\end{aligned}
\right]\,
\end{equation*}
Now compare the values and get the values of elements of L and U.
\end{frame}

\begin{frame}%{Example}
\begin{equation*}
L = \left[ \begin{aligned}
1 && 0 && 0 \\
3 && 1 && 0 \\
2 && 1 && 1
\end{aligned}
\right]\,,
U = \left[ \begin{aligned}
1 && 2 && 4 \\
0 && 2 && 2 \\
0 && 0 && 3
\end{aligned}
\right]\,.
\end{equation*}
The next step is to solve [L]\{y\}=\{b\} for the vector \{y\} that we consider
\begin{equation*}
Ly = \left[ \begin{aligned}
1 && 0 && 0 \\
3 && 1 && 0 \\
2 && 1 && 1
\end{aligned}
\right]\,*
\left[ \begin{aligned}
y_1 \\
y_2 \\
y_3
\end{aligned}
\right]\,=
\left[ \begin{aligned}
3 \\
13 \\
4
\end{aligned}
\right]\,=
b
\end{equation*}
which can be solved by forward substitution \{y\} = [3 4 -6$]^T$ now that we have found y we finish the procedure by solving
\begin{equation*}
Ux = \left[ \begin{aligned}
1 && 2 && 4 \\
0 && 2 && 2 \\
0 && 0 && 3
\end{aligned}
\right]\,*
\left[ \begin{aligned}
x_1 \\
x_2 \\
x_3
\end{aligned}
\right]\,=
\left[ \begin{aligned}
3 \\
4 \\
-6
\end{aligned}
\right]\,=
y
\end{equation*}
by using backward substitution we will get \{x\}.
\end{frame}

\section{Methods}
\begin{frame}{Algorithm}
%for j=1:n\\
%\hspace*{1cm}	for i=j:n\\
%\hspace*{1.5cm}	for k=0:i-1\\
%\hspace*{2cm}$L_{ik}U_{kj}$ = $A_{ij}$ gives row i of U\\
%\hspace*{1.5cm}	end\\
%\hspace*{1cm}	end\\
%\hspace*{1cm}	for j=i:n\\
%\hspace*{1.5cm}	for k=0:j-1\\
%\hspace*{2cm}$L_{ik}U_{kj}$ = $A_{ij}$ gives row i of L\\
%\hspace*{1.5cm}	end\\
%\hspace*{1cm}	end\\
%end	
\begin{center}
\begin{figure}[htp]
\centering
\includegraphics[scale=.4]{pic1.png}
\caption{Output}
\end{figure}
\end{center}
\end{frame}

\section{Tasks}
\begin{frame}{Task Generation and Dependency Graph}
\begin{figure}[htp]
\centering
\includegraphics[scale=.4]{pic2.png}
\caption{Output}
\end{figure}
\end{frame}

\section{Strategy}
\begin{frame}
Since the LU decomposition is completely done using elimination and substation, there are 3 for loops 
involved and also the cells of a particular row (for U) or particular column (for L) can be computed in 
parallel so we used LU decomposition block as a suitable area to implement parallelism. Each code has sufficient comments inside to describe the methods and important statements. 
\end{frame}

\begin{frame}{SpeedUp Table}
\begin{figure}[htp]
\centering
\includegraphics[scale=.4]{su.png}
\caption{SpeedUP Table}
\end{figure}
\end{frame}

\begin{frame}{SpeedUp Graph}
\begin{center}
\begin{figure}[htp]
\centering
\includegraphics[scale=.4]{spu.png}
\caption{SpeedUp Graph}
\end{figure}
\end{center}
\end{frame}

\begin{frame}{Performance}
\begin{figure}[htp]
\centering
\includegraphics[scale=.3]{pp.png}
\caption{No. of Threads vs. Time}
\end{figure}
\end{frame}

\begin{frame}{CPU Usage}
\begin{figure}[htp]
\centering
\includegraphics[scale=.4]{thr2.png}
\caption{For 2 threads}
\includegraphics[scale=.4]{thr_4.png}
\caption{For 4 threads}
\end{figure}
\end{frame}

\begin{frame}{Call Map}
\begin{figure}[htp]
\centering
\includegraphics[scale=.2]{call.png}
\caption{Callee Map for Parallel code}
\end{figure}
\end{frame}


\begin{frame}{Cache Misses}
\begin{figure}[htp]
\centering
\includegraphics[scale=.4]{cache.png}
\caption{Cache Misses}
\end{figure}
\end{frame}


\section{Q \& A}
\begin{frame}{Q \& A}
\begin{center}
Thank You!
\end{center}
\end{frame}

\end{document}